Util.v
@@ -1,13 +1,14 @@
 Require Import Coq.Setoids.Setoid.
 
 
+(* Relation classes *)
+
 Local Lemma R_refl [A] (R : relation A) (x y : A) (X : R x x) (E : x = y): R x y.
 Proof.
   rewrite <- E; apply X.
 Qed.
 
 Ltac reflexivityR := apply R_refl; reflexivity.
-
 
 Ltac symmetric_iff :=
   let H  := fresh "H"  in
@@ -20,6 +21,69 @@ Ltac symmetric_iff :=
            | eapply H; try solve [try symmetry; eassumption] ];
     clear H Hs
   ].
+
+Ltac auto_tc := auto with typeclass_instances.
+
+Module Rel.
+  Section Conj.
+    Context [A] (R0 R1 : relation A).
+
+    Definition conj : relation A := relation_conjunction R0 R1.
+    
+    Global Instance conj_Equivalence {E0 : Equivalence R0} {E1 : Equivalence R1}: Equivalence conj.
+    Proof.
+      split.
+      - intro x; split; reflexivity.
+      - intros x y []; split; symmetry; assumption.
+      - intros x y z [] []; split; etransitivity; eassumption.
+    Qed.
+
+    Global Instance conj_PreOrder {E0 : PreOrder R0} {E1 : PreOrder R1}: PreOrder conj.
+    Proof.
+      split.
+      - intro x; split; reflexivity.
+      - intros x y z [] []; split; etransitivity; eassumption.
+    Qed.
+  End Conj.
+  Section Point.
+    Context (A : Type) [B : Type] (R : relation B).
+
+    Definition point : relation (A -> B) := Morphisms.pointwise_relation A R.
+
+    Global Instance point_PreOrder {E : PreOrder R}: PreOrder point.
+    Proof.
+      split.
+      - intros x a; reflexivity.
+      - intros x y z H0 H1 a; etransitivity; eauto.
+    Qed.
+  End Point.
+  Section Pull.
+    Context [A B] (f : A -> B) (R : relation B).
+    
+    Definition pull : relation A := fun x y => R (f x) (f y).
+  
+    Global Instance pull_Equivalence {E : Equivalence R}: Equivalence pull.
+    Proof.
+      unfold pull; constructor; repeat intro.
+      - reflexivity.
+      - symmetry; auto.
+      - etransitivity; eauto.
+    Qed.
+    
+    Global Instance pull_PreOrder {E : PreOrder R}: PreOrder pull.
+    Proof.
+      unfold pull; constructor; repeat intro.
+      - reflexivity.
+      - etransitivity; eauto.
+    Qed.
+  End Pull.
+
+  Global Ltac by_expr E :=
+    match goal with
+    | |- _ ?R => change R with E; auto using Build_PreOrder with typeclass_instances
+    end.
+End Rel.
+
 
 (* [fset] *)
 
