Test/SLProg.v
@@ -26,8 +26,10 @@ Definition spec_aux_n (p : ptr) (n : nat) : Spec.t nat := {|
 Definition spec_aux : f_spec sig_aux :=
   fun p s => exists (n : nat), eq s (spec_aux_n p n).
 
-Definition spec_main_n (ps : ptr * ptr) : Spec.t unit := {|
-  Spec.pre  := SLprop.cell (fst ps) 0 ** SLprop.cell (snd ps) 0;
+Definition spec_main_n (ps : ptr * ptr) : Spec.t unit :=
+  let (p0, p1) := ps in {|
+  Spec.pre  := SLprop.ex nat (fun n0 => SLprop.cell p0 n0) **
+               SLprop.ex nat (fun n1 => SLprop.cell p1 n1);
   Spec.post := fun _ => SLprop.True;
 |}.
 
@@ -57,38 +59,46 @@ Definition impl_aux (p : ptr) : @CP.instr SIG nat :=
 
 Lemma sls_aux (p : ptr) (n : nat) : sls SPEC (impl_aux p) (spec_aux_n p n).
 Proof.
-  eapply Bind. eapply Read. intro n'.
-  eapply Cons. eapply Frame with (fr := SLprop.pure (n' = n)).
+  eapply Bind. eapply Read. intro n'; normalize.
+  apply PureE; intros ->.
   eapply Bind. eapply Write. intro _u.
-  eapply Ret with (sp := fun r => SLprop.cell p (n' + r)).
-  split; simpl.
-  - intros fm H.
-    assert (n' = n). {
-      case H as (? & ? & ? & ? & H); apply H.
-    }
-    subst n'; eassumption.
-  - intro r.
-    SLprop.normalize.
-    apply SLprop.imp_pure_l.
-    intros ->; reflexivity.
-Defined.
+  eapply Ret with (sp := fun r => SLprop.cell p (n + r)).
+Qed.
 
 Definition impl_main (ps : ptr * ptr) : @CP.instr SIG unit :=
   let (p0, p1) := ps in
-  CP.Bind (CP.Call (sg := sig_aux) f_aux eq_refl p0) (fun n =>
-  CP.Ret tt).
+  CP.Bind (CP.Read p1) (fun n1 =>
+  CP.Bind (CP.Call (sg := sig_aux) f_aux eq_refl p0) (fun m =>
+  CP.Bind (CP.Read p1) (fun n1' =>
+  sl_assert (SLprop.pure (n1 = n1'))))).
 
 Lemma sls_main ps : sls SPEC (impl_main ps) (spec_main_n ps).
 Proof.
   case ps as (p0, p1); simpl.
+  normalize.
+  eapply ExistsE; intro n0.
+  eapply ExistsE; intro n1.
   eapply Bind.
-  eapply Cons. eapply Frame with (fr := SLprop.cell p1 0).
-  eapply Call with (fs := call_aux p0 0).
-  reflexivityR.
-  intros _n.
-  eapply Cons. exact (Ret _ tt (fun _ => SLprop.True)).
-  split; simpl; constructor.
-Defined.
+    eapply CFrame with (fr := SLprop.cell p0 n0).
+    eapply Read.
+    simpl. rewrite SLprop.star_comm. reflexivityR.
+  intro; simpl; normalize; apply PureE; intros ->.
+  eapply Bind.
+    eapply CFrame with (fr := SLprop.cell p1 n1).
+    eapply Call with (fs := call_aux p0 n0).
+    rewrite SLprop.star_comm; reflexivityR.
+  intro m; simpl.
+  eapply Bind.
+    eapply CFrame with (fr := SLprop.cell p0 (n0 + m)).
+    eapply Read.
+    simpl. rewrite SLprop.star_comm. reflexivityR.
+  intro n1'; simpl; normalize; apply PureE; intros ->.
+    eapply CFrame.
+    apply Assert.
+  split; simpl.
+  - apply SLprop.imp_pure_r; reflexivity.
+  - constructor.
+Qed.
 
 Definition IMPL : CP.impl_context SIG :=
   fun f => match f with
@@ -101,11 +111,11 @@ Lemma match_context:
   CP.context_match_spec IMPL SPEC.
 Proof.
   intros [|[|]]; simpl. 3:constructor.
-  - intros p s TR.
-    apply tr_f_spec_exists in TR as [n TR].
-    refine (wp_impl_tr_f_spec TR).
+  - intro p; apply wp_impl_tr_f_spec.
+    intros ? [n ->].
     apply sls_aux.
   - intros ps; apply wp_impl_tr_f_spec.
+    intros ? ->.
     apply sls_main.
 Qed.
 
@@ -115,4 +125,28 @@ Proof.
   intros [|[|]]; simpl; repeat constructor.
   (* intro. set (imp := impl_main x); hnf in imp; subst imp. *)
   intros (?,?); simpl; repeat constructor.
+Qed.
+
+Lemma main_okstate m p0 p1 s'
+  (NN_P0  : p0 <> NULL) (NN_P1  : p1 <> NULL)
+  (NALIAS : p0 <> p1)
+  (STEPS  : CP.steps IMPL (m, CP.get_fun_body IMPL f_main eq_refl (p0, p1)) s'):
+  CP.okstate IMPL s'.
+Proof.
+  eapply CP.func_okstate in STEPS; eauto using match_context, context_oracle_free.
+  simpl; eexists _, SLprop.True; repeat esplit.
+  simpl.
+  eexists (fmem_of_mem m); split. apply match_fmem_of_mem.
+  ecase FMem.build_join as [fm0 FM0]; cycle 1.
+  eexists fm0, (fun p => if Mem.ptr_eq p p0 then None else if Mem.ptr_eq p p1 then None else Some (m p));
+    intuition; cycle 1.
+  - normalize; exists (m p0), (m p1).
+    simpl; eexists _, _; intuition; try reflexivity.
+    exact FM0.
+  - constructor.
+  - intro p; generalize (FM0 p); unfold FMem.cell.
+    do 2 case Mem.ptr_eq as [|]; simpl; subst;
+    simplify_eq 1; intros <-; reflexivity.
+  - intro p; unfold FMem.cell; simpl.
+    do 2 case Mem.ptr_eq as [|]; simpl; congruence.
 Qed.
